
       \question[4] Find the value of $a$ and $b$ if $(x-1)$ and $(x-2)$
       are factors of $x^3-ax+b$ ?
       \ifprintanswers
         \marginnote[2cm]{ We know that the unknown factor is of the form $(x-g)$
         because the coefficient of $x^3$ in the original equation is 1 }
         \marginnote{ Had the equation been $2x^3-ax+b$ or $3x^3-ax+b$, then the
         unknown term would have been $(2x-g)$ or $(3x-g)$, as the case may be}
       \fi 
       \begin{solution}[\halfpage]
          \begin{align}
            x^3-ax+b &= \overbrace{(x-1)\cdot(x-2)}^{\texttt{known factors}}\cdot
            \overbrace{(x-g)}^{\texttt{unknown factor}} \\
            &= (x^2-3x+2)\cdot(x-g) \\
            &= x^3-(g+3)x^2+(3g+2)x-2g
          \end{align}
        Comparing coefficients on both sides, we get: 
          \begin{align}
            g+3 &= 0 \Rightarrow g = -3\\ 
            3g+2 &= -a \Rightarrow a = 7\\
            -2g &= b  \Rightarrow b = 6
          \end{align} 
       \end{solution} 
       \ifprintanswers
          \marginnote[-2cm]{The original equation is therefore $x^3-7x+6$ and the 
          factors are $(x-1)$, $(x-2)$ and $(x+3)$}
        \fi
